template-coq/src/plugin_core.mli
@@ -8,6 +8,7 @@ type reduction_strategy = Redexpr.red_expr (* Template.TemplateMonad.Common.redu
 type global_reference = Names.GlobRef.t (* Template.Ast.global_reference *)
 type term = Constr.t  (* Template.Ast.term *)
 type mutual_inductive_body = Declarations.mutual_inductive_body (* Template.Ast.mutual_inductive_body *)
+type constant_body = Declarations.constant_body
 type constant_entry = Safe_typing.private_constants Entries.constant_entry (* Template.Ast.constant_entry *)
 type mutual_inductive_entry = Entries.mutual_inductive_entry (* Template.Ast.mutual_inductive_entry *)
 
@@ -49,7 +50,7 @@ val tmCurrentModPath : Names.ModPath.t tm
 
 val tmQuoteInductive : kername -> (Names.MutInd.t * mutual_inductive_body) option tm
 val tmQuoteUniverses : UGraph.t tm
-val tmQuoteConstant : kername -> bool -> constant_entry tm
+val tmQuoteConstant : kername -> bool -> constant_body tm
 
 val tmInductive : mutual_inductive_entry -> unit tm
 
