examples/demo.v
@@ -133,7 +133,8 @@ Definition mut_i : mutual_inductive_entry :=
   mind_entry_finite := Finite;
   mind_entry_params := [];
   mind_entry_inds := [one_i; one_i2];
-  mind_entry_universes := Monomorphic_ctx (LevelSet.empty, ConstraintSet.empty);
+  mind_entry_universes := Monomorphic_entry (LevelSet.empty, ConstraintSet.empty);
+  mind_entry_variance := None;
   mind_entry_private := None;
 |}.
 
@@ -158,9 +159,11 @@ Definition mut_list_i : mutual_inductive_entry :=
 {|
   mind_entry_record := None;
   mind_entry_finite := Finite;
-  mind_entry_params := [("A", LocalAssum (tSort Universe.type0))];
+  mind_entry_params := [{| decl_name := nNamed "A"; decl_body := None;
+                         decl_type := (tSort Universe.type0) |}];
   mind_entry_inds := [one_list_i];
-  mind_entry_universes := Monomorphic_ctx (LevelSet.empty, ConstraintSet.empty);
+  mind_entry_universes := Monomorphic_entry (LevelSet.empty, ConstraintSet.empty);
+  mind_entry_variance := None;
   mind_entry_private := None;
 |}.
 
@@ -183,9 +186,11 @@ Definition mut_pt_i : mutual_inductive_entry :=
 {|
   mind_entry_record := Some (Some "pp");
   mind_entry_finite := BiFinite;
-  mind_entry_params := [("A", LocalAssum (tSort Universe.type0))];
+  mind_entry_params := [{| decl_name := nNamed "A"; decl_body := None;
+                         decl_type := (tSort Universe.type0) |}];
   mind_entry_inds := [one_pt_i];
-  mind_entry_universes := Monomorphic_ctx (LevelSet.empty, ConstraintSet.empty);
+  mind_entry_universes := Monomorphic_entry (LevelSet.empty, ConstraintSet.empty);
+  mind_entry_variance := None;
   mind_entry_private := None;
 |}.
 
@@ -223,7 +228,7 @@ Qed.
 Run TemplateProgram ((tmQuoteConstant "six" true) >>= tmPrint).
 Run TemplateProgram ((tmQuoteConstant "six" false) >>= tmPrint).
 
-Run TemplateProgram (t <- tmLemma "foo4" nat ;;
+Run TemplateProgram (t <- tmLemma "foo4" nat;;
                      tmDefinition "foo5" (t + t + 2)).
 Next Obligation.
   exact 3.
