template-coq/theories/AstUtils.v
@@ -320,7 +320,7 @@ Fixpoint lookup_mind_decl (id : ident) (decls : global_env)
 
 Definition universes_entry_of_decl (u : universes_decl) : universes_entry :=
   match u with
-  | Polymorphic_ctx ctx => Polymorphic_entry (map nNamed (fst ctx)) (Universes.AUContext.repr ctx)
+  | Polymorphic_ctx ctx => Polymorphic_entry (fst ctx) (Universes.AUContext.repr ctx)
   | Monomorphic_ctx ctx => Monomorphic_entry ctx
   end.
 
@@ -330,11 +330,21 @@ Definition mind_body_to_entry (decl : mutual_inductive_body)
 Proof.
   refine {| mind_entry_record := None; (* not a record *)
             mind_entry_finite := Finite; (* inductive *)
-            mind_entry_params := decl.(ind_params);
+            mind_entry_params := _ (* Should be ind_params, but translations are broken: for Simon decl.(ind_params) *);
             mind_entry_inds := _;
             mind_entry_universes := universes_entry_of_decl decl.(ind_universes);
             mind_entry_variance := decl.(ind_variance);
             mind_entry_private := None |}.
+  - (* FIXME: this is wrong, the info should be in ind_params *)
+   refine (match List.hd_error decl.(ind_bodies) with
+  | Some i0 => List.rev _
+  | None => nil (* assert false: at least one inductive in a mutual block *)
+  end).
+  pose (typ := decompose_prod i0.(ind_type)).
+destruct typ as [[names types] _].
+apply (List.firstn decl.(ind_npars)) in names.
+apply (List.firstn decl.(ind_npars)) in types.
+  refine (map (fun '(x, ty) => vass x ty) (combine names types)).
   - refine (List.map _ decl.(ind_bodies)).
     intros [].
     refine {| mind_entry_typename := ind_name;
