template-coq/theories/TemplateMonad/Core.v
@@ -46,7 +46,7 @@ Cumulative Inductive TemplateMonad@{t u} : Type@{t} -> Prop :=
 (* Quote the body of a definition or inductive. Its name need not be fully qualified *)
 | tmQuoteInductive : qualid -> TemplateMonad mutual_inductive_body
 | tmQuoteUniverses : TemplateMonad constraints
-| tmQuoteConstant : qualid -> bool (* bypass opacity? *) -> TemplateMonad constant_entry
+| tmQuoteConstant : qualid -> bool (* bypass opacity? *) -> TemplateMonad constant_body
 (* unquote before making the definition *)
 (* FIXME take an optional universe context as well *)
 | tmMkInductive : mutual_inductive_entry -> TemplateMonad unit
